src/Bedrock/Field/FieldExtensions/QuadraticFieldExtensionsSpecs.v
@@ -1,8 +1,7 @@
 Require Import Rupicola.Lib.Api.
 (* Require Import Crypto.Arithmetic.PrimeFieldTheorems.
 Require Import Crypto.Arithmetic.FLia. *)
-Require Import Crypto.Bedrock.Specs.AbstractField.
-Require Import Crypto.Bedrock.Specs.PrimeField.
+Require Import Crypto.Bedrock.Specs.Field.
 Require Import Crypto.Bedrock.Field.Interface.Compilation2.
 Require Import Crypto.Bedrock.Field.FieldExtensions.Theory.QuadraticExtensions.
 Require Import Crypto.Arithmetic.PrimeFieldTheorems.
@@ -23,33 +22,21 @@ Section QuadraticExtension.
   Context {env_ok : map.ok env}.
   Context {ext_spec_ok : Semantics.ext_spec.ok ext_spec}.
 
-  Context {prime_field_parameters : PrimeFieldParameters}
-          {prime_field_parameters_ok : PrimeFieldParameters_ok}
+  Context {prime_parameters : PrimeParameters}
+          {prime_parameters_ok : PrimeParameters_ok}
           {M_mod : M_pos mod 4 =? 3 = true}.
+  Existing Instance prime_field_parameters.
+  Context {field_representation : FieldRepresentation (F M_pos)}
+          {field_representation_ok : FieldRepresentation_ok (F M_pos)}.
 
   Lemma M_big : 2 < M_pos.
   Proof.
     lia.
   Qed.
 
-  Local Instance F_parameters : FieldParameters.
-  Proof.
-    exact (PrimeField.prime_field_parameters).
-  Defined.
+  Local Notation Fp2 := ((F M_pos) * (F M_pos))%type.
 
-  Local Instance F_parameters_ok : FieldParameters_ok.
-  Proof.
-    constructor. destruct prime_field_parameters_ok.
-    apply (@F.field_modulo M_pos M_prime).
-  Qed.
-    
-
-  Context {F_representation : @FieldRepresentation F_parameters _ _ _ _}
-          {field_representation_ok : FieldRepresentation_ok}.
-
-  Definition prefix : string := "Fp2_".
-
-  Instance Fp2_parameters : FieldParameters.
+  Instance Fp2_parameters : FieldParameters Fp2.
   Proof.
       econstructor.
         - exact (zerop2 M_pos).
@@ -60,24 +47,11 @@ Section QuadraticExtension.
         - exact (subp2 M_pos).
         - exact (mulp2 M_pos).
         - exact (divp2 M_pos).
+        - exact (of_Zp2 M_pos).
         - eapply eq_dec_Fp2.
-        - exact (zerop2 M_pos). (*value of a_24, not relevant for BLS curves*)
-        - exact "Fp2_mul".
-        - exact "Fp2_add".
-        - exact "Fp2_sub".
-        - exact "Fp2_opp".
-        - exact "Fp2_square".
-        - exact "Fp2_scmula_24".
-        - exact "Fp2_inv".
-        - exact "Fp2_from_bytes".
-        - exact "Fp2_to_bytes".
-        - exact "Fp2_select".
-        - exact "Fp2_felem_copy".
-        - exact "Fp2_from_word".
-        - exact "Fp2_from_list".
   Defined.
 
-  Instance Fp2_parameters_ok : @FieldParameters_ok Fp2_parameters.
+  Instance Fp2_parameters_ok : FieldParameters_ok Fp2.
   Proof.
     econstructor;
     exact (@std_to_fiatCrypto_field _ _ _ _ _ _ _ _ _ (FFp2 M_pos M_prime M_big M_mod)).
@@ -89,7 +63,7 @@ Section QuadraticExtension.
   Definition fst_felem_bytes (Fp2_list : list byte) : list byte := firstn (Z.to_nat felem_size_in_bytes) Fp2_list.
   Definition snd_felem_bytes (Fp2_list : list byte) : list byte := skipn (Z.to_nat felem_size_in_bytes) Fp2_list.
 
-  Instance Fp2_representation : @FieldRepresentation Fp2_parameters _ _ _ _.
+  Instance Fp2_representation : FieldRepresentation Fp2.
   Proof.
     econstructor.
       - exact (fun y => (feval (fst_felem y), feval (snd_felem y))).
@@ -102,7 +76,7 @@ Section QuadraticExtension.
       - exact tight_bounds.
   Defined.
 
-  Instance Fp2_representation_ok : @FieldRepresentation_ok Fp2_parameters _ _ _ _ Fp2_representation.
+  Instance Fp2_representation_ok : FieldRepresentation_ok Fp2.
   Proof.
     econstructor; destruct field_representation_ok; intros.
     split; eapply relax_bounds; apply H.
